src/Std/Data/DTreeMap/Raw/Basic.lean
@@ -729,13 +729,13 @@ def inter (t₁ t₂ : Raw α β cmp) : Raw α β cmp :=
 instance : Inter (Raw α β cmp) := ⟨inter⟩
 
 /-- Internal implementation detail of the hash map. -/
-def beq [BEq α] [LawfulEqCmp cmp] [∀ k, BEq (β k)] (t₁ t₂ : Raw α β cmp) : Bool :=
+def beq [LawfulEqCmp cmp] [∀ k, BEq (β k)] (t₁ t₂ : Raw α β cmp) : Bool :=
   letI : Ord α := ⟨cmp⟩; t₁.inner.beq t₂.inner
 
-instance [BEq α] [LawfulEqCmp cmp] [∀ k, BEq (β k)] : BEq (Raw α β cmp) := ⟨beq⟩
+instance [LawfulEqCmp cmp] [∀ k, BEq (β k)] : BEq (Raw α β cmp) := ⟨beq⟩
 
 /-- Internal implementation detail of the hash map. -/
-def Const.beq {β : Type v} [BEq α] [BEq β] (t₁ t₂ : Raw α (fun _ => β) cmp) : Bool :=
+def Const.beq {β : Type v} [BEq β] (t₁ t₂ : Raw α (fun _ => β) cmp) : Bool :=
   letI : Ord α := ⟨cmp⟩; Internal.Impl.Const.beq t₁.inner t₂.inner
 
 @[inline, inherit_doc DTreeMap.eraseMany]
