src/Std/Data/DTreeMap/Lemmas.lean
@@ -2877,6 +2877,34 @@ theorem get!_inter_of_not_mem_left [TransCmp cmp] [Inhabited β]
 
 end Const
 
+section BEq
+variable {m₁ m₂ : DTreeMap α β cmp} [∀ k, BEq (β k)] [LawfulEqCmp cmp] [TransCmp cmp]
+
+theorem Equiv.beq [∀ k, ReflBEq (β k)] (h : m₁ ~m m₂) : m₁ == m₂ :=
+  Impl.Equiv.beq m₁.2 m₂.2 h.1
+
+theorem Equiv_of_beq_eq_true [∀ k, LawfulBEq (β k)] (h : m₁ == m₂) : m₁ ~m m₂ :=
+  ⟨@Impl.Equiv_of_beq_eq_true _ _ ⟨cmp⟩ m₁.1 m₂.1 _ _ _ _ m₁.2 m₂.2 h⟩
+
+theorem Equiv.beq_congr {m₃ m₄ : DTreeMap α β cmp} : m₁ ~m m₃ → m₂ ~m m₄ → (m₁ == m₂) = (m₃ == m₄) := fun h1 h2 =>
+  @Impl.Equiv.beq_congr _ _ ⟨cmp⟩ m₁.1 m₂.1 _ _ _ m₃.1 m₄.1 m₁.2 m₂.2 m₃.2 m₄.2 h1.1 h2.1
+
+end BEq
+
+section
+variable {β : Type v} {m₁ m₂ : DTreeMap α (fun _ => β) cmp} [BEq β]
+
+theorem Const.Equiv.beq [TransCmp cmp] [ReflBEq β] (h : m₁ ~m m₂) : DTreeMap.Const.beq m₁ m₂ := by
+  apply Impl.Const.Equiv.beq m₁.2 m₂.2 h.1
+
+theorem Const.Equiv_of_beq_eq_true [TransCmp cmp] [LawfulEqCmp cmp] [LawfulBEq β] (h : Const.beq m₁ m₂) : m₁ ~m m₂ :=
+  ⟨@Impl.Const.Equiv_of_beq_eq_true α ⟨cmp⟩ β m₁.1 m₂.1 _ _ _ _ m₁.2 m₂.2 h⟩
+
+theorem Const.Equiv.beq_congr [TransCmp cmp] [LawfulEqCmp cmp] {m₃ m₄ : DTreeMap α (fun _ => β) cmp} : m₁ ~m m₃ → m₂ ~m m₄ → Const.beq m₁ m₂ = Const.beq m₃ m₄ := fun h1 h2 =>
+  @Impl.Const.Equiv.beq_congr α ⟨cmp⟩ β m₁.1 m₂.1 _ _ m₃.1 m₄.1 _ m₁.2 m₂.2 m₃.2 m₄.2 h1.1 h2.1
+
+end
+
 section Alter
 
 theorem isEmpty_alter_eq_isEmpty_erase [TransCmp cmp] [LawfulEqCmp cmp] {k : α}
